src/program_proof/pav/server.v
@@ -6,8 +6,6 @@ From Perennial.program_proof Require Import std_proof.
 From iris.unstable.base_logic Require Import mono_list.
 From stdpp Require Import gmap.
 From Perennial.base_logic Require Import ghost_map.
-From RecordUpdate Require Import RecordSet.
-Import RecordSetNotations.
 
 Module hashChain.
 Record t :=
@@ -28,57 +26,56 @@ Module server.
 Record t :=
   mk {
     mu: loc;
-    trees: list (gmap (list w8) (list w8));
-    updates: gmap (list w8) (list w8);
-    chain: hashChain.t;
-    linkSigs: list (list w8);
     hon: bool;
     γmonoLinks: gname;
-    γmonoTrs: gname;
+    γmonoTrees: gname;
   }.
-#[global] Instance etaServer : Settable _ :=
-  settable! mk <mu; trees; updates; chain; linkSigs; hon; γmonoLinks; γmonoTrs>.
 
 Section local_defs.
 Context `{!heapGS Σ, !mono_listG (list w8) Σ, !mono_listG gname Σ, !ghost_mapG Σ (list w8) (list w8)}.
 
-Definition my_inv γmonoLinks γmonoTrs : iProp Σ :=
-  ∃ links γtrs trs updates prevLinks digs,
+Definition my_inv γmonoLinks γmonoTrees : iProp Σ :=
+  ∃ links γtrees trees updates prevLinks digs,
   "#Hbinds" ∷ ([∗ list] epoch ↦ xy; link ∈ (zip prevLinks digs); links,
     is_hash (chainSepSome.encodesF (chainSepSome.mk epoch xy.1 xy.2)) link) ∗
   "Hlinks" ∷ mono_list_auth_own γmonoLinks (1/2) links ∗
-  "Hmaps" ∷ ([∗ list] γtr; tr ∈ γtrs; (trs ++ [updates]), ghost_map_auth γtr (1/2) tr) ∗
-  "HmonoTrs" ∷ mono_list_auth_own γmonoTrs (1/2) γtrs ∗
-  "#Hdigs" ∷ ([∗ list] tr; dig ∈ trs; digs, isTreeDig tr dig).
+  "Htree_views" ∷ ([∗ list] γtr; tr ∈ γtrees; (trees ++ [updates]),
+    ghost_map_auth γtr (1/2) tr) ∗
+  "HmonoTrees" ∷ mono_list_auth_own γmonoTrees (1/2) γtrees ∗
+  "#Hdigs" ∷ ([∗ list] tr; dig ∈ trees; digs, isTreeDig tr dig).
 
 Definition own ptr obj : iProp Σ :=
-  ∃ sk sl_trees sl_treePtrs ptr_updates map_sl_updates sl_chain sl_linkSigs γtrs lastγTr,
+∃ sk sl_ptr_trees (ptr_trees : list loc) trees ptr_updates (updates : gmap (list w8) (list w8)) map_sl_updates sl_chain chain sl_linkSigs linkSigs γtrees,
   "Hsk" ∷ ptr ↦[server :: "sk"] (slice_val sk) ∗
-  "Hown_sk" ∷ own_sk sk (serv_sigpred obj.(γmonoLinks) obj.(γmonoTrs)) obj.(hon) ∗
+  "Hown_sk" ∷ own_sk sk (serv_sigpred obj.(γmonoLinks) obj.(γmonoTrees)) obj.(hon) ∗
   "Hchain" ∷ ptr ↦[server :: "chain"] (slice_val sl_chain) ∗
-  "Hown_chain" ∷ hashChain.own sl_chain obj.(chain) ∗
-  "HmonoLinks" ∷ mono_list_auth_own obj.(γmonoLinks) (1/2) obj.(chain).(hashChain.links) ∗
+  "Hown_chain" ∷ hashChain.own sl_chain chain ∗
+  "HmonoLinks" ∷ mono_list_auth_own obj.(γmonoLinks) (1/2) chain.(hashChain.links) ∗
   "HlinkSigs" ∷ ptr ↦[server :: "linkSigs"] (slice_val sl_linkSigs) ∗
-  "Hown_linkSigs" ∷ own_Slice2D sl_linkSigs (DfracOwn 1) obj.(linkSigs) ∗
-  (* Exists map from string IDs to slices s.t. the slices own the vals. *)
-  "Hmap_sl_updates" ∷ ([∗ map] sl_bytes; bytes ∈ map_sl_updates; (kmap bytes_to_string obj.(updates)),
+  "Hown_linkSigs" ∷ own_Slice2D sl_linkSigs (DfracOwn 1) linkSigs ∗
+
+  (* The latest updates. *)
+  (* Exists map of slices that own the respective vals. *)
+  "Hmap_sl_updates" ∷ ([∗ map] sl_bytes; bytes ∈ map_sl_updates; (kmap bytes_to_string updates),
     own_slice_small sl_bytes byteT (DfracOwn 1) bytes) ∗
   "Hown_updates" ∷ own_map ptr_updates (DfracOwn 1) map_sl_updates ∗
   "Hupdates" ∷ ptr ↦[server :: "updates"] #ptr_updates ∗
 
   (* Tree-specific stuff. *)
-  "Htrees" ∷ ptr ↦[server :: "trees"] (slice_val sl_trees) ∗
-  "Hsl_trees" ∷ own_slice_small sl_trees ptrT (DfracOwn 1) sl_treePtrs ∗
-  "Hown_trees" ∷ ([∗ list] ptr_tr; tr ∈ sl_treePtrs; obj.(trees),
+  "Htrees" ∷ ptr ↦[server :: "trees"] (slice_val sl_ptr_trees) ∗
+  "Hsl_ptr_trees" ∷ own_slice_small sl_ptr_trees ptrT (DfracOwn 1) ptr_trees ∗
+  "Hown_trees" ∷ ([∗ list] ptr_tr; tr ∈ ptr_trees; trees,
     own_Tree ptr_tr tr) ∗
-  "HmonoTrs" ∷ mono_list_auth_own obj.(γmonoTrs) (1/2) γtrs ∗
-  "%HlastγTr" ∷ ⌜Some lastγTr = last γtrs⌝ ∗
-  "Hview_updates" ∷ ghost_map_auth lastγTr (1/2) obj.(updates).
+  "HmonoTrees" ∷ mono_list_auth_own obj.(γmonoTrees) (1/2) γtrees ∗
+  (* Need view for latest tr to give put promises.
+     For other trees, views let us match up state with global inv. *)
+  "Htree_views" ∷ ([∗ list] γtr; tr ∈ γtrees; (trees ++ [updates]),
+    ghost_map_auth γtr (1/2) tr).
 
 Definition valid ptr obj : iProp Σ :=
   "#Hmu" ∷ ptr ↦[server :: "mu"]□ #obj.(mu) ∗
   "#HmuR" ∷ is_lock nroot #obj.(mu) (own ptr obj) ∗
-  "#Hinv" ∷ inv nroot (my_inv obj.(γmonoLinks) obj.(γmonoTrs)).
+  "#Hinv" ∷ inv nroot (my_inv obj.(γmonoLinks) obj.(γmonoTrees)).
 
 End local_defs.
 End server.
@@ -95,26 +92,85 @@ Record t :=
   }.
 
 Section local_defs.
-Context `{!heapGS Σ}.
+Context `{!heapGS Σ, !mono_listG (list w8) Σ, !mono_listG gname Σ, !ghost_mapG Σ (list w8) (list w8)}.
 
-Definition own ptr obj : iProp Σ :=
+Definition own ptr obj γmonoLinks γmonoTrees id val : iProp Σ :=
   ∃ sl_prev2Link sl_prevDig sl_linkSig sl_putSig d0 d1 d2 d3,
-  "HputEpoch" ∷ ptr ↦[servPutReply :: "putEpoch"] #obj.(putEpoch) ∗
-  "Hprev2Link" ∷ ptr ↦[servPutReply :: "prev2Link"] (slice_val sl_prev2Link) ∗
-  "Hsl_prev2Link" ∷ own_slice_small sl_prev2Link byteT d0 obj.(prev2Link) ∗
-  "HprevDig" ∷ ptr ↦[servPutReply :: "prevDig"] (slice_val sl_prevDig) ∗
-  "Hsl_prevDig" ∷ own_slice_small sl_prevDig byteT d1 obj.(prevDig) ∗
-  "HlinkSig" ∷ ptr ↦[servPutReply :: "linkSig"] (slice_val sl_linkSig) ∗
-  "Hsl_linkSig" ∷ own_slice_small sl_linkSig byteT d2 obj.(linkSig) ∗
-  "HputSig" ∷ ptr ↦[servPutReply :: "putSig"] (slice_val sl_putSig) ∗
-  "Hsl_putSig" ∷ own_slice_small sl_putSig byteT d3 obj.(putSig) ∗
-  "Herror" ∷ ptr ↦[servPutReply :: "error"] #obj.(error).
+  "Herror" ∷ ptr ↦[servPutReply :: "error"] #obj.(error) ∗
+  if negb obj.(error) then
+    "HputEpoch" ∷ ptr ↦[servPutReply :: "putEpoch"] #obj.(putEpoch) ∗
+    "Hprev2Link" ∷ ptr ↦[servPutReply :: "prev2Link"] (slice_val sl_prev2Link) ∗
+    "Hsl_prev2Link" ∷ own_slice_small sl_prev2Link byteT d0 obj.(prev2Link) ∗
+    "HprevDig" ∷ ptr ↦[servPutReply :: "prevDig"] (slice_val sl_prevDig) ∗
+    "Hsl_prevDig" ∷ own_slice_small sl_prevDig byteT d1 obj.(prevDig) ∗
+    "HlinkSig" ∷ ptr ↦[servPutReply :: "linkSig"] (slice_val sl_linkSig) ∗
+    "Hsl_linkSig" ∷ own_slice_small sl_linkSig byteT d2 obj.(linkSig) ∗
+    "HputSig" ∷ ptr ↦[servPutReply :: "putSig"] (slice_val sl_putSig) ∗
+    "Hsl_putSig" ∷ own_slice_small sl_putSig byteT d3 obj.(putSig) ∗
+    (* Valid sigpreds, proving that the server completed the op. *)
+    "Hlink_sigpred" ∷ serv_sigpred_link γmonoLinks (servSepLink.mk obj.(prev2Link)) ∗
+    "Hput_sigpred" ∷ serv_sigpred_put γmonoTrees (servSepPut.mk obj.(putEpoch) id val)
+  else True.
 
 End local_defs.
 End servPutReply.
 
 Section proofs.
 Context `{!heapGS Σ, !mono_listG (list w8) Σ, !mono_listG gname Σ, !ghost_mapG Σ (list w8) (list w8)}.
+
+Lemma sep_auth_agree γtrees trees0 trees1 :
+  ([∗ list] γtr;tr ∈ γtrees;trees0, ghost_map_auth γtr (1/2) tr) -∗
+  ([∗ list] γtr;tr ∈ γtrees;trees1, ghost_map_auth γtr (1/2) tr) -∗
+  ⌜trees0 = trees1⌝.
+Proof.
+  iIntros "Hsep0 Hsep1".
+  unfold_leibniz.
+  setoid_rewrite list_equiv_lookup.
+  fold_leibniz.
+  iDestruct (big_sepL2_length with "Hsep0") as %Hlen0.
+  iDestruct (big_sepL2_length with "Hsep1") as %Hlen1.
+  iIntros (i).
+  destruct (decide (i < length γtrees)) as [Hbound | Hbound].
+  {
+    apply lookup_lt_is_Some in Hbound as [x0 Hlook0].
+    iDestruct (big_sepL2_lookup_1_some with "Hsep0") as %[x1 Hlook1]; [done|].
+    iDestruct (big_sepL2_lookup_1_some with "Hsep1") as %[x2 Hlook2]; [done|].
+    iDestruct (big_sepL2_lookup with "Hsep0") as "Hauth0"; [done..|].
+    iDestruct (big_sepL2_lookup with "Hsep1") as "Hauth1"; [done..|].
+    iDestruct (ghost_map_auth_agree with "Hauth0 Hauth1") as %->.
+    rewrite Hlook1 Hlook2.
+    done.
+  }
+  {
+    assert (trees0 !! i = None) as ->.
+    { apply lookup_ge_None; lia. }
+    assert (trees1 !! i = None) as ->.
+    { apply lookup_ge_None; lia. }
+done.
+  }
+Qed.
+
+Lemma inv_open_unify γmonoLinks links γmonoTrees γtrees trees updates :
+  mono_list_auth_own γmonoLinks (1/2) links -∗
+  mono_list_auth_own γmonoTrees (1/2) γtrees -∗
+  ([∗ list] γtr; tr ∈ γtrees; (trees ++ [updates]),
+    ghost_map_auth γtr (1/2) tr) -∗
+  inv nroot (server.my_inv γmonoLinks γmonoTrees) -∗
+  |={⊤}=>
+  ∃ prevLinks digs,
+  "#Hbinds" ∷ ([∗ list] epoch ↦ xy; link ∈ (zip prevLinks digs); links,
+    is_hash (chainSepSome.encodesF (chainSepSome.mk epoch xy.1 xy.2)) link) ∗
+  "#Hdigs" ∷ ([∗ list] tr; dig ∈ trees; digs, isTreeDig tr dig).
+Proof.
+  iIntros "Hlinks0 HmonoTrees0 Htree_views0 Hinv".
+  iInv "Hinv" as "> Hinv" "Hclose"; iNamed "Hinv".
+  iDestruct (mono_list_auth_own_agree with "Hlinks Hlinks0") as %[_ ->].
+  iDestruct (mono_list_auth_own_agree with "HmonoTrees HmonoTrees0") as %[_ ->].
+  iDestruct (sep_auth_agree with "Htree_views Htree_views0") as %?; list_simplifier.
+  iFrame "#".
+  iMod ("Hclose" with "[$]") as "_".
+  done.
+Qed.
 
 Lemma wp_server_put ptr_serv obj_serv sl_id sl_val (id val : list w8) d0 d1 :
   {{{
@@ -125,11 +181,7 @@ Lemma wp_server_put ptr_serv obj_serv sl_id sl_val (id val : list w8) d0 d1 :
   server__put #ptr_serv (slice_val sl_id) (slice_val sl_val)
   {{{
     ptr_reply reply, RET #ptr_reply;
-    "Hreply" ∷ servPutReply.own ptr_reply reply ∗
-    if negb reply.(servPutReply.error) then
-      "Hserv" ∷ server.valid ptr_serv (obj_serv <|server.updates := (<[id:=val]>obj_serv.(server.updates))|>)
-    else
-      "Hserv" ∷ server.valid ptr_serv obj_serv
+    "Hreply" ∷ servPutReply.own ptr_reply reply obj_serv.(server.γmonoLinks) obj_serv.(server.γmonoTrees) id val
   }}}.
 Proof.
   rewrite /server__put.
@@ -142,23 +194,15 @@ Proof.
     iIntros (ptr_errReply) "Hptr_errReply".
   iDestruct (struct_fields_split with "Hptr_errReply") as "H"; iNamed "H".
   wp_storeField.
-  iAssert (servPutReply.own ptr_errReply _) with "[putEpoch prev2Link prevDig linkSig putSig error]" as "HerrReply".
-  {
-    instantiate (1:=servPutReply.mk _ _ _ _ _ _).
-    rewrite /servPutReply.own /=.
-    iExists Slice.nil, Slice.nil, Slice.nil, Slice.nil.
-    iDestruct (own_slice_zero byteT (DfracOwn 1)) as "H0".
-    iDestruct (own_slice_to_small with "H0") as "H1".
-    iFrame "#∗".
-  }
+  iAssert (servPutReply.own ptr_errReply (servPutReply.mk 0 [] [] [] [] _) obj_serv.(server.γmonoLinks) obj_serv.(server.γmonoTrees) id val) with "[$error //]" as "HerrReply".
 
-  (* check id len *)
+  (* check id len. *)
   wp_apply wp_slice_len.
   wp_if_destruct.
   {
     wp_loadField.
     wp_apply (release_spec with "[-HΦ HerrReply]"); [iFrame "#∗%"|].
-    wp_pures; iApply "HΦ"; by iFrame "∗#".
+    wp_pures; by iApply "HΦ".
   }
 
   (* check if id was already updated. if not, update. *)
@@ -170,7 +214,7 @@ Proof.
   {
     wp_loadField.
     wp_apply (release_spec with "[-HΦ HerrReply]"); [iFrame "#∗%"|].
-    wp_pures; iApply "HΦ"; by iFrame "∗#".
+    wp_pures; by iApply "HΦ".
   }
   wp_loadField.
   wp_apply (wp_MapInsert_to_val with "[$Hown_updates]"); iIntros "Hown_updates".
@@ -191,29 +235,77 @@ Proof.
     iRename "Hobj" into "Hptr_putPre";
     iRename "Hsl_enc" into "Hsl_putPre";
     move: Henc => Henc_putPre.
+  replace (word.add (word.sub sl_ptr_trees.(Slice.sz) (W64 1)) (W64 1)) with (sl_ptr_trees.(Slice.sz)) in Henc_putPre by ring.
+
+  (* get resources for put promise. *)
+  (* get mono_list_idx_own. *)
+  iDestruct (own_slice_small_sz with "Hsl_ptr_trees") as %Hlen0.
+  iDestruct (big_sepL2_length with "Hown_trees") as %Hlen1.
+  iDestruct (big_sepL2_length with "Htree_views") as %Hlen2.
+  rewrite app_length/= in Hlen2.
+  assert (uint.nat sl_ptr_trees.(Slice.sz) < length γtrees) as Hinb by lia.
+  apply lookup_lt_is_Some in Hinb as [γtree Hlook0].
+  iDestruct (mono_list_idx_own_get with "[HmonoTrees]") as "#Hidx_γtree".
+  2: iApply (mono_list_lb_own_get with "HmonoTrees").
+  1: done.
+  (* get ghost map witness by opening invariant. *)
+  wp_apply ncfupd_wp.
+  iRename "HmonoTrees" into "HmonoTrees0".
+  iRename "Htree_views" into "Htree_views0".
+  iInv "Hinv" as "> H" "Hclose"; iNamed "H".
+  iDestruct (mono_list_auth_own_agree with "HmonoTrees HmonoTrees0") as %[_ ->].
+  iDestruct (sep_auth_agree with "Htree_views Htree_views0") as %?; list_simplifier.
+  assert ((trees ++ [updates]) !! uint.nat sl_ptr_trees.(Slice.sz) = Some updates) as Hlook1.
+  { apply lookup_snoc_Some; eauto with lia. }
+  iDestruct (big_sepL2_insert_acc with "Htree_views0") as "[Hmap_auth0 Hsep_close0]"; [done..|].
+  iDestruct (big_sepL2_insert_acc with "Htree_views") as "[Hmap_auth1 Hsep_close1]"; [done..|].
+  iCombine "Hmap_auth0 Hmap_auth1" as "Hmap_auth".
+  apply map_get_false in Hmap_get as [Hmap_get _].
+  iDestruct (big_sepM2_lookup_l_none with "Hmap_sl_updates") as "%Hmap_get1"; [done|].
+  rewrite lookup_kmap in Hmap_get1.
+  iMod (ghost_map_insert_persist _ val with "Hmap_auth") as "[[Hmap_auth0 Hmap_auth1] #Hwitness]"; [done|].
+  (* make resources look pretty before closing invariant. *)
+  iDestruct ("Hsep_close0" with "Hmap_auth0") as "Htree_views0".
+  iDestruct ("Hsep_close1" with "Hmap_auth1") as "Htree_views1".
+  pose proof (list_insert_id _ _ _ Hlook0) as H;
+    iEval (rewrite H) in "Htree_views0 Htree_views1";
+    clear H.
+  assert (uint.nat sl_ptr_trees.(Slice.sz) = length trees + 0) as H by lia;
+    iEval (rewrite H insert_app_r) in "Htree_views0 Htree_views1";
+    list_simplifier; clear H.
+  iMod ("Hclose" with "[$Hlinks $HmonoTrees $Htree_views1]") as "_"; [iFrame "#"|].
 
   (* sign put promise. *)
-  (* use iInv to open invariant to get other half of ghost_map. *)
-  About ghost_map_insert.
-  iMod (ghost_map_insert with "[$Hview_updates]").
-  Print map_get.
-  Search map_get.
-  apply map_get_false in Hmap_get as [Hmap_get _].
+  iModIntro.
   wp_loadField.
   wp_apply (wp_Sign with "[$Hown_sk $Hsl_putPre]").
   {
+    iRight.
+    (* TODO: with iFrame "%", it's unfolding mono_list_idx_own,
+       framing the lookup, and left with a mono_list_lb_own, which we don't have.
+       maybe mono_list_idx_own should be more opaque? *)
+    iFrame (Henc_putPre).
+    iFrame "#".
+  }
+  iIntros (sl_sig sig) "H";
+    iRename "Hsk" into "Hptr_sk";
+    iNamed "H";
+    iRename "Hmsg" into "Hsl_putPre";
+    iRename "Hsig" into "HputSig".
 
-    rewrite /serv_sigpred.
-    Print serv_sigpred_put.
-    (* for serv_sigpred_put:
-       need to give idx_own Trs for epoch. and persis ghost_map ptsto.
-       should already have idx_own. at prev updateEpoch, we expanded mono_list.
-       need to iMod ghost_map to give persis thing.
-    *)
-    iEval 
-    }
+  (* get all the other data to be returned. *)
+  wp_loadField.
+  Print serv_sigpred_link.
+  (*
+     what are we returning here?
+     at prev epoch update, we committed a new link.
+     there's an invariance that is_hash holds true for some stuff.
+     also that isTreeDig holds true, so that's what we used.
+     and direct hashChain inv is that mono_list_auth of all this.
+  *)
+  Search hashChain__getLink.
+
 Admitted.
-*)
 
 Lemma wp_server_updateEpoch ptr_serv obj_serv :
   {{{
